books/cutil/define.lisp
@@ -17,42 +17,19 @@
 ; Foundation, Inc., 51 Franklin Street, Suite 500, Boston, MA 02110-1335, USA.
 ;
 ; Original author: Jared Davis <jared@centtech.com>
+; Modified by David Rager <ragerdl@cs.utexas.edu> to add :assert option
+; Modified by Sol Swords <sswords@centtech.com> to add untranslate support
 
 (in-package "CUTIL")
-(include-book "defaggregate")
-(include-book "deflist")
-(include-book "defprojection")
+(include-book "formals")
+(include-book "returnspecs")
 (include-book "xdoc-impl/fmt-to-str" :dir :system)
 (include-book "tools/mv-nth" :dir :system)
+(include-book "str/cat" :dir :system)
 (set-state-ok t)
+(program)
 
-(defun interactive-p (state)
-  (declare (xargs :mode :program))
-  (not (f-get-global 'acl2::certify-book-info state)))
-
-(make-event
-
-; I originally wrote this file in logic mode.  You'll see theorems below, etc.
-; But there is a problem:
-;
-;   - End-users (including me) would much rather have all this stuff in program
-;     mode.  They don't care a lick about reasoning about cutil::formal-p and
-;     that sort of thing, and we don't want theorems about the guts of define
-;     messing with real proofs.
-;
-;   - Developers (including me) would much rather have all this stuff in logic
-;     mode.  They want verified guards, assertions to be checked, etc.
-;
-; So, as a dumb hack: if we're aren't certifying a book, then do everything in
-; logic mode to make sure the guards get checked.  If we're certifying the book,
-; do it in program-mode so none of these theorems actually get exported.
-
- (if (interactive-p state)
-     (value '(value-triple :invisible))
-   (value '(program))))
-
-(local (include-book "misc/assert" :dir :system))
-(local (include-book "system/legal-variablep" :dir :system))
+(include-book "misc/assert" :dir :system)
 
 (defxdoc define
   :parents (cutil)
@@ -60,13 +37,13 @@
 
   :long "<h3>Introduction</h3>
 
-<p>@('define') is an extension of @('defun')/@('defund') with:</p>
+<p>@('define') is an extension of @('defun')/@('defun') with:</p>
 
 <ul>
 
-<li>Richer @('formals') lists that permit keyword/optional arguments and
-embedded guards and documentation, and which automatically infer @(see stobj)
-declarations and <b>BOZO FUTURE WORK</b> some type declarations.</li>
+<li>Richer @('formals') lists that permit keyword/optional arguments, embedded
+guards and documentation, automatically infer @(see stobj) declarations,
+etc.</li>
 
 <li>A more concise @(see xargs) syntax that also adds control over other
 settings like @(see set-ignore-ok), @(see set-irrelevant-formals-ok), and
@@ -97,95 +74,7 @@ in the body.</li>
 function to be defined, as in @(see defun).  The other parts all have their own
 syntax and features to cover, and we address them in turn.</p>
 
-
-<h3>The Formals</h3>
-
-<p>The @('formals') syntax is a proper extension of the normal formals for a
-@(see defun).  That is, you can still use a plain list of variable names.  In
-this case, the only new feature of @('define') is that it automatically
-determines which formals are @(see stobjs) and generates an appropriate
-@('(declare (xargs :stobjs ...))') form.  But there are also some more
-interesting extensions.</p>
-
-<h4>Keyword and Optional Arguments</h4>
-
-<p>You can also use @('&key') and @('&optional') as in @(see macro-args).
-Other lambda-list keywords like @('&rest') aren't supported.</p>
-
-<p>When @('define') sees these keywords, then instead of just producing a
-@('defun') it will generate:</p>
-
-<ul>
-<li>A function, @('name-fn'),</li>
-<li>A wrapper macro, @('name'),</li>
-<li>A <see topic='@(url macro-aliases-table)'>macro alias</see> associating
-@('name-fn') with @('name')</li>
-</ul>
-
-<h4>Embedded Guards and Documentation</h4>
-
-<p>Beyond just naming the formals, you can specify simple guards for them and
-document them right in the formals list.  Here is an example:</p>
-
-@({
- (define split-up-string
-   ((x stringp \"The string to split\")
-    (separators (and (consp separators)
-                     (character-listp separators))
-     \"What letters to split on -- <b>dropped from the result!</b>\")
-    &key
-    (limit natp
-     \"Where to stop, typically @('nil') which means @('(length x)')\"))
-   ...)
-})
-
-<p>The general form for an extended formal is:</p>
-
-@({
-     (varname [guard] [xdoc])     i.e., both the guard and xdoc are optional
-  OR (varname [xdoc] [guard])           and may be given in any order
-})
-
-<p>As a convenient shorthand, the @('guard') may be a single symbol, e.g.,
-above the guard for @('x') is @('(stringp x)').  To be more precise:</p>
-
-<ul>
- <li>@('t') and @('nil') are treated literally, and</li>
- <li>Any other symbol @('g') is treated as short for @('(g var)')</li>
-</ul>
-
-<p>Aside for future expansion: a nice side-effect of this treatment is that a
-keyword like @(':foo') will produce the guard @('(:foo var)') which is invalid
-and hence will be rejected.  So, if we eventually want to add keyword arguments
-to our formals syntax, we'll be able to do that.</p>
-
-<p>For more complex guards, you can also write down arbitrary terms, e.g.,
-above @('separators') must be a non-empty character list.  We require that such
-a guard be at least a cons to distinguish it from documentation and symbol
-guards.  We also require that it is not simply a quoted constant.  This ensures
-that guards can be distinguished from default values in macro arguments.  For
-example, compare:</p>
-
-@({
-     &key (x 'atom)     ;; x has no guard, default value 'atom
- vs. &key (x atom)      ;; x has guard (atom x), default value nil
- vs. &key ((x atom) '3) ;; x has guard (atom x), default value 3
-})
-
-<p>BOZO this is not yet implemented.  Eventually I want it to be true: As a
-special convenience, certain guards like @('stringp') and @('(unsigned-byte-p
-32 x)'), are recognized as @(see type-spec)s and result in @(see type)
-declarations for the Lisp compiler.  This may occasionally improve efficiency.
-Note that this is a very limited mechanism and it can easily fail to add
-declarations that are trivially implied by the guard.</p>
-
-<p>The @('xdoc') is any string.  It will be embedded within the within @(see
-xdoc) documentation, so you may make use of @(see xdoc::markup) and @(see
-xdoc::preprocessor) directives.  Typically these descriptions should be short
-and not include document-structuring tags like @('<p>'), @('<ul>'), @('<h3>'),
-and so forth.  See the section on xdoc integration, below, for more
-details.</p>
-
+<p>The formal have many features; see @(see extended-formals).</p>
 
 <h3>The Main Stuff</h3>
 
@@ -312,97 +201,7 @@ needed for termination.</dd>
 
 <h4>@('Returns') Specifications</h4>
 
-<p>A more elaborate extended option is @(':returns').  This is a concise way to
-name, document, and prove basic type-like theorems about the return values of
-your functions.  The general form is:</p>
-
-@({
-    :returns return-spec       ;; for single-value functions
- or :returns (mv return-spec*) ;; for multiple-valued functions
-})
-
-<p>There should be exactly one @('return-spec') per return value.  Each
-return-spec has the form:</p>
-
-@({
-     name               ;; just for naming return values
-  or (name [option]*)   ;; for naming, documenting, and proving theorems
-})
-
-<p>where @('name') is a symbol and the options can come in any order.  To
-distinguish between the two forms of @(':returns'), it is not legal to use
-@('mv') as the name of a return value.  The options are:</p>
-
-<dl>
-
-<dt>@('<xdoc>'), any string literal</dt>
-
-<dd>You can document each return value with a string literal.  The string may
-make use of @(see xdoc::markup) and @(see xdoc::preprocessor) directives.
-Typically these descriptions should be short and not include
-document-structuring tags like @('<p>'), @('<ul>'), @('<h3>'), and so forth.
-See the section on xdoc integration, below, for more details.</dd>
-
-<dt>@('<return-type>'), a symbol or term</dt>
-
-<dd>When provided, the return type is used to generate a basic type-like
-theorems about the return values.</dd>
-
-<dd><b>Important Note</b> in the multiple-valued case, this approach assumes
-you are using the @('tools/mv-nth') book.  The theorems we prove target terms
-like @('(mv-nth 0 (f ...))') and @('(mv-nth 1 (f ...))').  This will not work
-well if @(see mv-nth) is enabled, especially about the 0th return value. For
-your convenience, @('define') automatically includes the @('tools/mv-nth')
-book.  You really should be using it, you know.</dd>
-
-<dd>As a convenient shorthand, you can use a single symbol like @('evenp').
-The theorem to be proven in this case might be, e.g., @('(evenp (f x))') for a
-single-valued function, or @('(evenp (mv-nth 3 (f x)))') if this is the
-fourth (because of zero-indexing) return value of a multiply-valued function.
-The symbol @('t') is explicitly allowed and results in no theorem.  The symbol
-@('nil') and keyword symbols are explicitly invalid as return types.</dd>
-
-<dd>In certain cases, you may wish to prove a more complex theorem, e.g., say
-we want to prove this return value is always greater than 5.  To support this,
-you can write a return type like @('(< 5 ans)'), where @('ans') is the
-@('name') of this return value.  You can also refer to the names of other
-return values in this term.  To make it easy to distinguish return types from
-other options, the return type term must be a cons and must not begin with
-@('quote').</dd>
-
-<dt>@(':hyp hyp-term')</dt>
-
-<dd>This option only makes sense when there is a return-type term.  By default,
-the return-type theorem is unconditional.  If the theorem needs a hypothesis,
-you can put it here.</dd>
-
-<dd>Frequently, the hypothesis you want for a type-like theorem is for the
-guards of the function to be met.  As a convenient shorthand, @('hyp-term') may
-be:
-
-<ul>
-<li>@(':guard') -- use the function's guard as the hypothesis</li>
-<li>@(':fguard') -- like @(':guard'), but @(see force) the entire guard</li>
-</ul>
-
-If neither of these is what you want, you can provide an arbitrary
-@('hyp-term').  Typically this term should mention only the formals of your
-function.  The return values of the theorem will not be bound in scope of the
-hyp, so trying to refer to them in a hypothesis is generally an error.</dd>
-
-<dt>@(':hints hints-term')</dt>
-
-<dd>This option only makes sense when there is a return-type term.  By default,
-this is @('nil'), but when specified, the hints are passed to the proof attempt
-for the associated return-type.</dd>
-
-<dt>@(':rule-classes classes')</dt>
-
-<dd>This option only makes sense when there is a return-type term.  By default,
-the return-type theorem is added as a @(':rewrite') rule.  If you want to use
-other @(see rule-classes), then you will want to override this default.</dd>
-
-</dl>
+<p>See @(see returns-specifiers)</p>
 
 <h4>@('Assert') Specification</h4>
 
@@ -466,486 +265,9 @@ some kind of separator!</p>
 ")
 
 
-; Preliminaries ---------------------------------------------------------------
 
 
 
-
-; Trivial lemmas...
-
-(local (defthm consp-of-assoc-equal
-         (implies (alistp alist)
-                  (equal (consp (assoc-equal key alist))
-                         (if (assoc-equal key alist)
-                             t
-                           nil)))
-         :hints(("Goal" :in-theory (enable assoc-equal)))))
-
-(local (defthm alistp-of-delete-assoc
-         (implies (alistp alist)
-                  (alistp (delete-assoc key alist)))))
-
-(local (defthm stringp-of-car-when-string-listp
-         (implies (string-listp x)
-                  (equal (stringp (car x))
-                         (consp x)))))
-
-
-; World Inspection ------------------------------------------------------------
-
-(defsection var-is-stobj-p
-
-  (defund var-is-stobj-p (var world)
-    (declare (xargs :guard (and (symbolp var)
-                                (plist-worldp world))))
-    (consp (getprop var 'acl2::stobj nil 'current-acl2-world world)))
-
-  (local
-   (progn
-     (assert! (not (var-is-stobj-p 'foo (w state))))
-     (assert! (var-is-stobj-p 'state (w state)))
-     (defstobj foo (field1 :initially 0))
-     (assert! (var-is-stobj-p 'foo (w state))))))
-
-(defsection look-up-formals
-
-  (defund look-up-formals (fn world)
-    (declare (xargs :guard (and (symbolp fn)
-                                (plist-worldp world))))
-    (b* ((look (getprop fn 'acl2::formals :bad 'acl2::current-acl2-world world))
-         ((when (eq look :bad))
-          (er hard? 'look-up-formals
-              "Can't look up the formals for ~x0!" fn))
-         ((unless (symbol-listp look))
-          (er hard? 'look-up-formals
-              "Expected a symbol-listp, but found ~x0!" look)))
-      look))
-
-  (local (in-theory (enable look-up-formals)))
-
-  (defthm symbol-listp-of-look-up-formals
-    (symbol-listp (look-up-formals fn world)))
-
-  (local
-   (progn
-    (assert! (equal (look-up-formals 'look-up-formals (w state))
-                    '(fn world))))))
-
-(defsection look-up-guard
-
-  (defund look-up-guard (fn world)
-    (declare (xargs :guard (and (symbolp fn)
-                                (plist-worldp world))))
-    (b* ((?tmp
-          ;; Silly... make sure the function exists, causing an error
-          ;; otherwise.
-          (look-up-formals fn world)))
-      (getprop fn 'acl2::guard t 'acl2::current-acl2-world world)))
-
-  (local
-   (progn
-   (defun f1 (x) x)
-   (defun f2 (x) (declare (xargs :guard (natp x))) x)
-   (defun f3 (x) (declare (xargs :guard (and (integerp x)
-                                             (<= 3 x)
-                                             (<= x 13))))
-     x)
-   (assert! (equal (look-up-guard 'f1 (w state)) 't))
-   (assert! (equal (look-up-guard 'f2 (w state)) '(natp x)))
-   (assert! (equal (look-up-guard 'f3 (w state))
-                   '(IF (INTEGERP X)
-                        (IF (NOT (< X '3)) (NOT (< '13 X)) 'NIL)
-                        'NIL))))))
-
-(defsection look-up-return-vals
-
-  ;; Returns the stobjs-out property, a list that may have NILs and stobj names
-  ;; with the same length as the number of return vals for FN.
-
-  (defund look-up-return-vals (fn world)
-    (declare (xargs :guard (and (symbolp fn)
-                                (plist-worldp world))))
-    (b* ((stobjs-out
-          (getprop fn 'acl2::stobjs-out :bad 'acl2::current-acl2-world world))
-         ((when (eq stobjs-out :bad))
-          (er hard? 'look-up-return-vals
-              "Can't look up stobjs-out for ~x0!" fn)
-          '(NIL))
-         ((unless (and (consp stobjs-out)
-                       (symbol-listp stobjs-out)))
-          (er hard? 'look-up-return-vals
-              "Expected stobjs-out to be a non-empty symbol-list, but found ~x0."
-              stobjs-out)
-          '(NIL)))
-      stobjs-out))
-
-  (local (in-theory (enable look-up-return-vals)))
-
-  (defthm symbol-listp-of-look-up-return-vals
-    (symbol-listp (look-up-return-vals fn world)))
-
-  (local
-   (progn
-     (defun f1 (x) x)
-     (defun f2 (x) (mv x x))
-     (defun f3 (x state) (declare (xargs :stobjs state)) (mv x state))
-     (assert! (equal (look-up-return-vals 'f1 (w state)) '(nil)))
-     (assert! (equal (look-up-return-vals 'f2 (w state)) '(nil nil)))
-     (assert! (equal (look-up-return-vals 'f3 (w state)) '(nil state))))))
-
-
-(defsection look-up-wrapper-args
-
-; Like look-up-formals, except that wrapper can be a function or a macro.
-
-  (defund look-up-wrapper-args (wrapper world)
-    (declare (xargs :guard (and (symbolp wrapper)
-                                (plist-worldp world))))
-    (b* ((look (getprop wrapper 'acl2::formals :bad
-                        'acl2::current-acl2-world world))
-         ((unless (eq look :bad))
-          look)
-         (look (getprop wrapper 'acl2::macro-args :bad
-                        'acl2::current-acl2-world world))
-         ((unless (eq look :bad))
-          look))
-      (er hard? 'look-up-wrapper-args
-          "Failed to find formals or macro-args for ~x0!" wrapper)))
-  (local
-   (progn
-     (defun f1 (x) x)
-     (defmacro f2 (x) x)
-     (defmacro f3 (x y &key (c '5) (d '7)) (list x y c d))
-     (assert! (equal (look-up-wrapper-args 'f1 (w state)) '(x)))
-     (assert! (equal (look-up-wrapper-args 'f2 (w state)) '(x)))
-     (assert! (equal (look-up-wrapper-args 'f3 (w state))
-                     '(x y &key (c '5) (d '7)))))))
-
-
-
-; -------------- Formals Stuff ------------------------------------------------
-
-(defaggregate formal
-  (name
-   guard   ; always a term, t for formals with no guard
-   doc     ; always a string, "" for formals with no documentation
-   )
-  :tag :formal
-  :require ((legal-variablep-of-formal->name
-             (legal-variablep name))
-            (stringp-of-vl-formal->doc
-             (stringp doc)
-             :rule-classes :type-prescription)))
-
-(deflist formallist-p (x)
-  (formal-p x)
-  :elementp-of-nil nil)
-
-(defund parse-formal-name (fnname varname)
-  (declare (xargs :guard t))
-  (b* (((when (legal-variablep varname))
-        varname)
-       (fake-arglist (list varname))
-       ((when (acl2::arglistp fake-arglist))
-        (er hard? 'parse-formal-name
-            "Error in ~x0: formal ~x1: mysterious problem that Jared thinks ~
-             should be impossible, please tell him that he is wrong."
-            fnname varname)
-        'default-valid-legal-variablep)
-       ((mv & reason)
-        ;; BOZO should be able to get rid of this ec-call if someone can
-        ;; verify the guards of find-first-bad-arg.
-        (ec-call (acl2::find-first-bad-arg fake-arglist))))
-    (er hard? 'parse-formal-name
-        "Error in ~x0: formal ~x1 is invalid: ~s2." fnname varname reason)
-    'default-valid-legal-variablep))
-
-(defthm legal-variablep-of-parse-formal-name
-  (legal-variablep (parse-formal-name fnname varname))
-  :hints(("Goal" :in-theory (enable parse-formal-name))))
-
-(defund parse-formal-item (fnname varname item guards docs)
-  "Returns (mv guards docs)"
-  (declare (xargs :guard (legal-variablep varname)))
-  (cond ((booleanp item)
-         (mv (cons item guards) docs))
-        ((symbolp item)
-         (mv (cons `(,item ,varname) guards) docs))
-        ((and (consp item)
-              (not (eq (car item) 'quote)))
-         (mv (cons item guards) docs))
-        ((stringp item)
-         (mv guards (cons item docs)))
-        (t
-         (progn$
-          (er hard? 'parse-formal-item
-              "Error in ~x0, formal ~x1: expected guard specifiers or ~
-               documentation strings, but found ~x2."
-              fnname varname item)
-          (mv guards docs)))))
-
-(defthm string-listp-of-parse-formal-item-1
-  (implies (string-listp docs)
-           (b* (((mv ?guards docs)
-                 (parse-formal-item fnname varname items guards docs)))
-             (string-listp docs)))
-  :hints(("Goal" :in-theory (enable parse-formal-item))))
-
-(defund parse-formal-items (fnname varname items guards docs)
-  "Returns (mv guards docs)"
-  (declare (xargs :guard (legal-variablep varname)))
-  (b* (((when (not items)) (mv guards docs))
-       ((when (atom items))
-        (er hard? 'parse-formal-items
-            "Error in ~x0: expected formal-items to be nil-terminated, ~
-             but found ~x1 as the final cdr." fnname items)
-        (mv guards docs))
-       ((mv guards docs)
-        (parse-formal-item fnname varname (car items) guards docs)))
-    (parse-formal-items fnname varname (cdr items) guards docs)))
-
-(defthm string-listp-of-parse-formal-items-1
-  (implies (string-listp docs)
-           (b* (((mv ?guards docs)
-                 (parse-formal-items fnname varname items guards docs)))
-             (string-listp docs)))
-  :hints(("Goal" :in-theory (enable parse-formal-items))))
-
-(defund parse-formal (fnname formal)
-  "Returns a formal-p"
-  (declare (xargs :guard t))
-  (b* (((when (atom formal))
-        (b* ((varname (parse-formal-name fnname formal)))
-          (make-formal :name varname
-                       :guard t
-                       :doc "")))
-       (varname (parse-formal-name fnname (car formal)))
-       (items   (cdr formal))
-       ((mv guards docs) (parse-formal-items fnname varname items nil nil))
-       (guard (cond ((atom guards) 't)
-                    ((eql (len guards) 1) (car guards))
-                    (t (er hard? 'parse-formal
-                           "Error in ~x0, formal ~x1: expected a single guard ~
-                            term, but found ~&2." fnname varname guards))))
-       (doc   (cond ((atom docs) "")
-                    ((eql (len docs) 1) (car docs))
-                    (t (progn$
-                        (er hard? 'parse-formal
-                            "Error in ~x0, formal ~x1: expected a single xdoc ~
-                             string, but found ~&2." fnname varname docs)
-                        "")))))
-    (make-formal :name varname
-                 :guard guard
-                 :doc doc)))
-
-(defthm formal-p-of-parse-formal
-  (formal-p (parse-formal fnname formal))
-  :hints(("Goal" :in-theory (enable parse-formal))))
-
-(defund parse-formals (fnname formals)
-  ;; Assumes lambda-list keywords have already been removed from formals.
-  (declare (xargs :guard t))
-  (b* (((when (not formals))
-        nil)
-       ((when (atom formals))
-        (er hard? 'parse-formals
-            "Error in ~x0: expected formals to be nil-terminated, but found ~
-             ~x1 as the final cdr." fnname formals)))
-    (cons (parse-formal fnname (car formals))
-          (parse-formals fnname (cdr formals)))))
-
-(defthm formallist-p-of-parse-formals
-  (formallist-p (parse-formals fnname formals))
-  :hints(("Goal" :in-theory (enable parse-formals))))
-
-(defprojection formallist->names (x)
-  (formal->name x)
-  :guard (formallist-p x)
-  :nil-preservingp t
-  :optimize nil)
-
-(defprojection formallist->guards (x)
-  (formal->guard x)
-  :guard (formallist-p x)
-  :nil-preservingp t
-  :optimize nil)
-
-(defund formallist-collect-stobjs (x world)
-  (declare (xargs :guard (and (formallist-p x)
-                              (plist-worldp world))))
-  (cond ((atom x)
-         nil)
-        ((var-is-stobj-p (formal->name (car x)) world)
-         (cons (car x) (formallist-collect-stobjs (cdr x) world)))
-        (t
-         (formallist-collect-stobjs (cdr x) world))))
-
-(defthm formallist-p-of-formallist-collect-stobjs
-  (implies (formallist-p x)
-           (formallist-p (formallist-collect-stobjs x world)))
-  :hints(("Goal" :in-theory (enable formallist-collect-stobjs))))
-
-
-
-
-; -------------- Macro Formals Support ----------------------------------------
-
-(defund has-macro-args (x)
-  (declare (xargs :guard t))
-  (if (atom x)
-      nil
-    (or (acl2::lambda-keywordp (car x))
-        (has-macro-args (cdr x)))))
-
-(defund remove-macro-args (fnname formals seenp)
-  ;; Generates a new list of (unparsed) formals, with the macro arguments
-  ;; removed.  This is going to be the list of formals for the -fn.  We are
-  ;; going to remove "&key" and "&optional" from formals, and also fix up
-  ;; any keyword/optional formals that have default values.
-  ;;
-  ;; When an argument has a default value it looks like
-  ;;   (foo 'default).
-  ;; The quote here distinguishes it from an extended formal that has a guard,
-  ;; e.g., (foo 'atom) has a default value of 'atom and no guard, whereas
-  ;; (foo atom) is just a plain extended formal with no default value (well, a
-  ;; default value of nil) and a guard of (atom foo).
-  ;;
-  ;; Seenp says whether we've seen &key or &optional yet.  Until we've seen one
-  ;; of these we don't change anything.
-  (declare (xargs :guard t))
-  (b* (((when (atom formals))
-        formals)
-       ((cons arg1 rest) formals)
-       ((when (or (eq arg1 '&key)
-                  (eq arg1 '&optional)))
-        (remove-macro-args fnname rest t))
-       ((when (acl2::lambda-keywordp arg1))
-        (er hard? 'remove-macro-args
-            "Error in ~x0: ~x1 only supports &key and &optional macro-style ~
-             arguments, but found ~x2." fnname 'define arg1))
-       ((unless seenp)
-        ;; Haven't yet seen &key/&optional, so don't change any args yet.
-        (cons arg1 (remove-macro-args fnname rest seenp)))
-
-       ;; Saw &keyword/&optional already and this isn't another keyword.  So,
-       ;; this is a real keyword/optional argument.  We need to remove any
-       ;; default value.
-       ((when (and (consp arg1)
-                   (true-listp arg1)
-                   (equal (len arg1) 2)
-                   (consp (second arg1))
-                   (eq (car (second arg1)) 'quote)))
-        ;; Arg1 matches (foo 'value), so it has a default value to remove.
-        ;; Change it to drop the default value.
-        (cons (first arg1) (remove-macro-args fnname rest seenp))))
-
-    ;; Else, it doesn't match (foo 'value), so leave it alone.
-    (cons arg1 (remove-macro-args fnname rest seenp))))
-
-(local
- (progn
-   (assert! (equal (remove-macro-args 'f '(a b c) nil)
-                   '(a b c)))
-   (assert! (equal (remove-macro-args 'f '(a b c &key d e) nil)
-                   '(a b c d e)))
-   (assert! (equal (remove-macro-args 'f '(a b c &key d &optional e) nil)
-                   '(a b c d e)))
-   (assert! (equal (remove-macro-args 'f '(a b c &optional d e) nil)
-                   '(a b c d e)))
-   (assert! (equal (remove-macro-args 'f '(a b c &key (d true-listp) e) nil)
-                   ;; true-listp is unquoted so it's a guard
-                   '(a b c (d true-listp) e)))
-   (assert! (equal (remove-macro-args 'f '(a b c &key (d 'true-listp) e) nil)
-                   ;; 'true-listp is quoted so it's a default value
-                   '(a b c d e)))
-   (assert! (equal (remove-macro-args 'f '(a b c &key (d "foo") e) nil)
-                   ;; "foo" is unquoted so it's an xdoc string
-                   '(a b c (d "foo") e)))
-   (assert! (equal (remove-macro-args 'f '(a b c &key (d '"foo") e) nil)
-                   ;; '"foo" is quoted so it's a default value
-                   '(a b c d e)))
-   (assert! (equal (remove-macro-args 'f '(a b c &key ((d atom) '3) (e true-listp)) nil)
-                   '(a b c (d atom) (e true-listp))))))
-
-
-(defund formals-for-macro (fnname formals seenp)
-  ;; Remove extended formal stuff (guards, documentation) and just get down to
-  ;; a list of variable names and &key/&optional stuff.  This will be the
-  ;; formals for the wrapper macro.
-  (declare (xargs :guard t))
-  (b* (((when (atom formals))
-        formals)
-       ((cons arg1 rest) formals)
-       ((when (or (eq arg1 '&key)
-                  (eq arg1 '&optional)))
-        (cons arg1 (formals-for-macro fnname rest t)))
-       ((when (acl2::lambda-keywordp arg1))
-        (er hard? 'formals-for-macro
-            "Error in ~x0: ~x1 only supports &key and &optional macro-style ~
-             arguments, but found ~x2." fnname 'define arg1))
-
-       ((unless seenp)
-        ;; Haven't yet seen &key/&optional, so the only args should be ordinary
-        ;; symbols and extended formals.  Keep just the name.  If it's a
-        ;; extended formal then it has the form (name ...).
-        (cons (if (atom arg1) arg1 (car arg1))
-              (formals-for-macro fnname rest seenp)))
-
-       ;; Saw &keyword/&optional already and this isn't another keyword.  So,
-       ;; this is a real keyword/optional argument.  If there's a default value
-       ;; we need to keep it.
-       ((when (and (consp arg1)
-                   (true-listp arg1)
-                   (equal (len arg1) 2)
-                   (consp (second arg1))
-                   (eq (car (second arg1)) 'quote)))
-        ;; Arg1 matches (extended-formal 'value).  We need to keep just
-        ;; (name 'value)
-        (let* ((eformal     (first arg1))
-               (default-val (second arg1)) ;; already quoted
-               (name        (if (atom eformal) eformal (car eformal))))
-          (cons (list name default-val)
-                (formals-for-macro fnname rest seenp)))))
-
-    ;; Else, it doesn't match (foo 'value), so just do the name extraction like
-    ;; normal.
-    (cons (if (atom arg1) arg1 (car arg1))
-          (formals-for-macro fnname rest seenp))))
-
-(local
- (progn
-   (assert! (equal (formals-for-macro 'f '(a b c) nil)
-                   '(a b c)))
-   (assert! (equal (formals-for-macro 'f '(a b c &key d e) nil)
-                   '(a b c &key d e)))
-   (assert! (equal (formals-for-macro 'f '(a b c &key d &optional e) nil)
-                   '(a b c &key d &optional e)))
-   (assert! (equal (formals-for-macro 'f '(a b c &optional d e) nil)
-                   '(a b c &optional d e)))
-   (assert! (equal (formals-for-macro 'f '(a b c &key (d true-listp) e) nil)
-                   ;; true-listp is unquoted so it's a guard
-                   '(a b c &key d e)))
-   (assert! (equal (formals-for-macro 'f '(a b c &key (d 'true-listp) e) nil)
-                   ;; 'true-listp is quoted so it's a default value
-                   '(a b c &key (d 'true-listp) e)))
-   (assert! (equal (formals-for-macro 'f '(a b c &key (d "foo") e) nil)
-                   ;; "foo" is unquoted so it's an xdoc string
-                   '(a b c &key d e)))
-   (assert! (equal (formals-for-macro 'f '(a b c &key (d '"foo") e) nil)
-                   ;; '"foo" is quoted so it's a default value
-                   '(a b c &key (d '"foo") e)))
-   (assert! (equal (formals-for-macro 'f '(a b c &key ((d atom) '3) (e true-listp)) nil)
-                   '(a b c &key (d '3) e)))))
-
-(defun make-wrapper-macro (fnname fnname-fn formals)
-  (declare (xargs :guard (and (symbolp fnname)
-                              (symbolp fnname-fn))))
-  (b* ((fn-formals     (remove-macro-args fnname formals nil))
-       (macro-formals  (formals-for-macro fnname formals nil))
-       (parsed-formals (parse-formals fnname fn-formals))
-       (fn-arg-names   (formallist->names parsed-formals)))
-    `(defmacro ,fnname ,macro-formals
-       (list ',fnname-fn . ,fn-arg-names))))
 
 ; -------------- Assertion Specifications -------------------------------------
 
@@ -959,7 +281,7 @@ some kind of separator!</p>
 ; could be used twice.  I'm not fixing this for now, because really we should
 ; be using the returns specifications, and doing so will obviate this issue.
 
-        (t (cons `(if (,(car assertion) ,(car assertion)) 
+        (t (cons `(if (,(car assertion) ,(car assertion))
                       t
                     (er hard? ',ctx
                         "Assertion failure.  The following was supposed to ~
@@ -968,460 +290,10 @@ some kind of separator!</p>
                         ,(car assertion)))
                  (parse-assert-tests (cdr assertion) ctx)))))
 
-; -------------- Returns Specifications ---------------------------------------
-
-(defaggregate returnspec
-  (name
-   doc           ; "" when omitted
-   return-type   ; t when omitted
-   hyp           ; t when omitted
-   hints         ; nil when omitted
-   rule-classes  ; :rewrite when omitted
-   )
-  :tag :return-spec
-  :require ((symbolp-of-returnspec->name
-             (symbolp name)
-             :rule-classes :type-prescription)
-            (stringp-of-returnspec->doc
-             (stringp doc)
-             :rule-classes :type-prescription)))
-
-(deflist returnspeclist-p (x)
-  (returnspec-p x)
-  :elementp-of-nil nil)
-
-(defconst *default-returnspec*
-  (make-returnspec :name 'ret
-                   :doc ""
-                   :return-type t
-                   :hyp t
-                   :hints nil
-                   :rule-classes :rewrite))
-
-(defund extract-keywords (fnname legal-kwds args kwd-alist)
-  "Returns (mv kwd-alist other-args)"
-  (declare (xargs :guard (and (symbol-listp legal-kwds)
-                              (no-duplicatesp legal-kwds)
-                              (alistp kwd-alist))))
-  (b* (((when (atom args))
-        (mv kwd-alist args))
-       (arg1 (first args))
-       ((when (keywordp arg1))
-        (b* (((unless (member arg1 legal-kwds))
-              (er hard? 'extract-keyword-aux
-                  "Error in ~x0: invalid keyword ~x1." fnname arg1)
-              (mv nil nil))
-             ((when (atom (rest args)))
-              (er hard? 'extract-keywords
-                  "Error in ~x0: expected keyword ~x1 to be followed by an ~
-                   argument." fnname arg1)
-              (mv nil nil))
-             ((when (assoc arg1 kwd-alist))
-              (er hard? 'extract-keywords
-                  "Error in ~x0: found multiple occurrences of keyword ~x1."
-                  fnname arg1)
-              (mv nil nil))
-             (value (second args))
-             (kwd-alist (acons arg1 value kwd-alist)))
-          (extract-keywords fnname legal-kwds (cddr args) kwd-alist)))
-       ((mv kwd-alist other-args)
-        (extract-keywords fnname legal-kwds (cdr args) kwd-alist)))
-    (mv kwd-alist (cons arg1 other-args))))
-
-(defthm true-listp-of-extract-keywords
-  (implies (true-listp args)
-           (true-listp
-            (mv-nth 1 (extract-keywords fnname legal-kwds args kwd-alist))))
-  :rule-classes :type-prescription
-  :hints(("Goal" :in-theory (enable extract-keywords))))
-
-(defthm alistp-of-extract-keywords
-  (implies (force (alistp kwd-alist))
-           (b* (((mv kwd-alist ?other-args)
-                 (extract-keywords fnname legal-kwds args kwd-alist)))
-             (alistp kwd-alist)))
-  :hints(("Goal" :in-theory (enable extract-keywords))))
-
-(defund parse-returnspec-item (fnname varname item terms docs)
-  "Returns (mv terms docs)"
-  (declare (xargs :guard t))
-  (cond ((eq item t)
-         ;; T is explicitly allowed as a return type
-         (mv (cons item terms) docs))
-        ((or (eq item nil)
-             (keywordp item))
-         (progn$
-         ;; NIL/keywords are explicitly not allowed
-          (er hard? 'parse-returnspec-item
-              "Error in ~x0: return type for ~x1 is ~x2, which is ~
-              not allowed." fnname varname item)
-          (mv terms docs)))
-        ((symbolp item)
-         (mv (cons `(,item ,varname) terms) docs))
-        ((and (consp item)
-              (not (eq (car item) 'quote)))
-         (mv (cons item terms) docs))
-        ((stringp item)
-         (mv terms (cons item docs)))
-        (t
-         (progn$
-          (er hard? 'parse-returnspec-item
-              "Error in ~x0, return type for ~x1: expected return ~
-               type terms or documentation strings, but found ~x2."
-              fnname varname item)
-          (mv terms docs)))))
-
-(defthm string-listp-of-parse-returnspec-item
-  (implies (string-listp docs)
-           (b* (((mv ?terms docs)
-                 (parse-returnspec-item fnname varname items terms docs)))
-             (string-listp docs)))
-  :hints(("Goal" :in-theory (enable parse-returnspec-item))))
-
-(defund parse-returnspec-items (fnname varname items terms docs)
-  "Returns (mv terms docs)"
-  (declare (xargs :guard t))
-  (b* (((when (not items))
-        (mv terms docs))
-       ((when (atom items))
-        (er hard? 'parse-returnspec-items
-            "Error in ~x0: expected returnspec-items for ~x1 to be ~
-             nil-terminated, but found ~x2 as the final cdr."
-            fnname varname items)
-        (mv terms docs))
-       ((mv terms docs)
-        (parse-returnspec-item fnname varname (car items) terms docs)))
-    (parse-returnspec-items fnname varname (cdr items) terms docs)))
-
-(defthm string-listp-of-parse-returnspec-items
-  (implies (string-listp docs)
-           (b* (((mv ?terms docs)
-                 (parse-returnspec-items fnname varname items terms docs)))
-             (string-listp docs)))
-  :hints(("Goal" :in-theory (enable parse-returnspec-items))))
-
-(defund parse-returnspec (fnname x world)
-  (declare (xargs :guard (plist-worldp world)))
-  (b* (((when (eq x 'mv))
-        (er hard? 'parse-returnspec
-            "Error in ~x0: return values may not be named MV."
-            fnname)
-        *default-returnspec*)
-       ((when (symbolp x))
-        ;; Fine, just a name, no docs/type
-        ;; Someone once got very confused why :returns character-listp
-        ;; wasn't proving that his function wasn't returning a character
-        ;; list.  So, now, make sure this isn't a defined function.
-        (b* ((look (getprop x 'acl2::formals :bad
-                            'acl2::current-acl2-world world))
-             ((unless (eq look :bad))
-              (er hard? 'parse-returnspec
-                  "Error in ~x0: you named a return value ~x1, which is ~
-                   is the name of a defined function, but you don't have ~
-                   any return type associated with this value.  There's a ~
-                   good chance this you meant this to be the return value's ~
-                   type instead of its name.~%~%~
-                   If you really want to name this return value ~x1 and ~
-                   not prove anything about it, you can use syntax like ~
-                   ~x2.~%"
-                  fnname x (list x t))
-              *default-returnspec*))
-          ;; Else, seems fine, just a name.
-          (make-returnspec :name x
-                           :doc ""
-                           :return-type t
-                           :rule-classes :rewrite
-                           :hyp nil
-                           :hints nil)))
-       ((when (atom x))
-        (er hard? 'parse-returnspec
-            "Error in ~x0: return specifiers must be symbols or lists, but ~
-             found: ~x1" fnname x)
-        *default-returnspec*)
-       ((cons varname options) x)
-       ((unless (symbolp varname))
-        (er hard? 'parse-returnspec
-            "Error in ~x0: return specifiers must start with a symbol name, ~
-             so this return specifier is not valid: ~x1" fnname x)
-        *default-returnspec*)
-       ((when (eq varname 'mv))
-        (er hard? 'parse-returnspec
-            "Error in ~x0: return values may not be named MV." fnname)
-        *default-returnspec*)
-
-       ((mv kwd-alist other-opts)
-        ;; bozo better context for error message here would be good
-        (extract-keywords fnname '(:hyp :hints :rule-classes) options nil))
-       (hyp (if (assoc :hyp kwd-alist)
-                (cdr (assoc :hyp kwd-alist))
-              t))
-       (hints (if (assoc :hints kwd-alist)
-                (cdr (assoc :hints kwd-alist))
-              nil))
-       (rule-classes (if (assoc :rule-classes kwd-alist)
-                         (cdr (assoc :rule-classes kwd-alist))
-                       :rewrite))
-       ((mv terms docs)
-        (parse-returnspec-items fnname varname other-opts nil nil))
-       (return-type
-        (cond ((atom terms) ;; no return-type terms, fine, default is t
-               t)
-              ((atom (cdr terms))
-               (car terms))
-              (t
-               (er hard? 'parse-returnspec
-                   "Error in ~x0: return specifier ~x1 has multiple return ~
-                    type terms, but at most one is allowed: ~&2"
-                   fnname varname terms))))
-       (xdoc
-        (cond ((atom docs) ;; no documentation, go figure, default is ""
-               "")
-              ((atom (cdr docs))
-               (car docs))
-              (t
-               (progn$
-                (er hard? 'parse-returnspec
-                    "Error in ~x0: return specifier ~x1 has multiple xdoc ~
-                     strings, but at most one is allowed: ~x2."
-                    fnname varname terms)
-                "")))))
-    (make-returnspec :name varname
-                      :doc xdoc
-                      :return-type return-type
-                      :rule-classes rule-classes
-                      :hyp hyp
-                      :hints hints)))
-
-(defthm returnspec-p-of-parse-returnspec
-  (returnspec-p (parse-returnspec fnname x world))
-  :hints(("Goal" :in-theory (enable parse-returnspec))))
-
-(defund parse-returnspecs-aux (fnname x world)
-  ;; Assumes they've already been normalized...
-  (declare (xargs :guard (plist-worldp world)))
-  (if (atom x)
-      nil
-    (cons (parse-returnspec fnname (car x) world)
-          (parse-returnspecs-aux fnname (cdr x) world))))
-
-(defthm returnspeclist-p-of-parse-returnspecs-aux
-  (returnspeclist-p (parse-returnspecs-aux fnname x world))
-  :hints(("Goal" :in-theory (enable parse-returnspecs-aux))))
-
-(defund normalize-returnspecs (fnname x)
-  ;; We support two forms of returns:
-  ;;  :returns return-spec
-  ;;  :returns (mv return-spec ... return-spec)
-  ;; We require that names are never MV, so we can just check for MV to
-  ;; tell thich kind of return spec we are dealing with.
-  ;; This function just converts either form into a list of return specs
-  ;; with no MV part.
-  (declare (xargs :guard t))
-  (cond ((not x)
-         ;; Fine, no return spec
-         nil)
-        ((eq x 'mv)
-         (er hard? 'normalize-returnspecs
-             "Error in ~x0: :returns may not be just MV." fnname))
-        ((symbolp x)
-         ;; Fine
-         (list x))
-        ((atom x)
-         (er hard? 'normalize-returnspecs
-             "Error in ~x0: :returns may not be ~x1."
-             fnname x))
-        ((eq (car x) 'mv)
-         (if (true-listp (cdr x))
-             (cdr x)
-           (er hard? 'normalize-returnspecs
-               "Error in ~x0: :returns must be nil-terminated."
-               fnname x)))
-        (t
-         (list x))))
-
-(defund parse-returnspecs (fnname x world)
-  (declare (xargs :guard (plist-worldp world)))
-  (parse-returnspecs-aux fnname
-                         (normalize-returnspecs fnname x)
-                         world))
-
-(defthm returnspeclist-p-of-parse-returnspecs
-  (returnspeclist-p (parse-returnspecs fnname x world))
-  :hints(("Goal" :in-theory (enable parse-returnspecs))))
-
-(defsection untranslate-and
-
-  (defund untranslate-and (x)
-    (declare (xargs :guard t))
-    (cond ((atom x)
-           ;; (and x) --> x
-           (list x))
-          ((and (consp x)
-                (eq (first x) 'if)
-                (equal (len x) 4)
-                (equal (fourth x) ''nil))
-           ;; (and x y ...) --> (if x (and y ...) nil)
-           (cons (second x)
-                 (untranslate-and (third x))))
-          (t
-           (list x))))
-
-  (local
-   (progn
-     (assert! (equal (untranslate-and 'x) '(x)))
-     (assert! (equal (untranslate-and 't) '(t)))
-     (assert! (equal (untranslate-and '(if x y z)) '((if x y z))))
-     (assert! (equal (untranslate-and '(if x y 'nil)) '(x y)))
-     (assert! (equal (untranslate-and '(if x (if a b c) 'nil)) '(x (if a b c))))
-     (assert! (equal (untranslate-and '(if x (if a b 'nil) 'nil)) '(x a b))))))
-
-(defund force-each (x)
-  (declare (xargs :guard t))
-  (if (atom x)
-      nil
-    (cons `(force ,(car x))
-          (force-each (cdr x)))))
-
-(defund fancy-force-hyp (x)
-  (declare (xargs :guard t))
-  (b* ((hyp-list (untranslate-and x)))
-    (cons 'and (force-each hyp-list))))
-
-(defund fancy-hyp (x)
-  (declare (xargs :guard t))
-  (b* ((hyp-list (untranslate-and x)))
-    (cons 'and hyp-list)))
-
-(defund returnspec-single-thm (fnname x world)
-  "Returns EVENTS"
-  ;; Only valid to call AFTER the function has been submitted, because we look
-  ;; up the guard/formals from the world.
-  (declare (xargs :guard (and (symbolp fnname)
-                              (returnspec-p x)
-                              (plist-worldp world))))
-  (b* (((returnspec x) x)
-       ((when (equal x.return-type t))
-        nil)
-       (formals (look-up-formals fnname world))
-       (hyp     (cond ((eq x.hyp :guard)
-                       (fancy-hyp (look-up-guard fnname world)))
-                      ((eq x.hyp :fguard)
-                       (fancy-force-hyp (look-up-guard fnname world)))
-                      (t
-                       x.hyp)))
-       (hints x.hints)
-       (concl   `(let ((,x.name (,fnname . ,formals)))
-                   ,x.return-type))
-       (formula (if (eq hyp t)
-                    concl
-                  `(implies ,hyp ,concl))))
-    `((defthm ,(intern-in-package-of-symbol
-                (concatenate 'string "RETURN-TYPE-OF-" (symbol-name fnname))
-                fnname)
-        ,formula
-        :hints ,hints
-        :rule-classes ,x.rule-classes))))
-
-(defund returnspec-multi-thm (fnname binds x world)
-  "Returns EVENTS"
-  (declare (xargs :guard (and (symbolp fnname)
-                              (returnspec-p x)
-                              (plist-worldp world))))
-  (b* (((returnspec x) x)
-       ((when (equal x.return-type t))
-        nil)
-       (hyp (cond
-             ((eq x.hyp :guard) (fancy-hyp (look-up-guard fnname world)))
-             ((eq x.hyp :fguard) (fancy-force-hyp (look-up-guard fnname world)))
-             (t x.hyp)))
-
-       (hints x.hints)
-       (concl `(b* (,binds)
-                 ,x.return-type))
-       (formula (if (eq hyp t)
-                    concl
-                  `(implies ,hyp ,concl))))
-    `((defthm ,(intern-in-package-of-symbol
-                (concatenate 'string "RETURN-TYPE-OF-" (symbol-name fnname)
-                             "." (symbol-name x.name))
-                fnname)
-        ,formula
-        :hints ,hints
-        :rule-classes ,x.rule-classes))))
-
-(defund returnspec-multi-thms (fnname binds x world)
-  "Returns EVENTS"
-  (declare (xargs :guard (and (symbolp fnname)
-                              (returnspeclist-p x)
-                              (plist-worldp world))))
-  (if (atom x)
-      nil
-    (append (returnspec-multi-thm fnname binds (car x) world)
-            (returnspec-multi-thms fnname binds (cdr x) world))))
-
-(defprojection returnspeclist->names (x)
-  (returnspec->name x)
-  :guard (returnspeclist-p x)
-  :result-type symbol-listp
-  :optimize nil)
-
-(defund make-symbol-ignorable (x)
-  (declare (xargs :guard (symbolp x)))
-  (intern-in-package-of-symbol
-   (concatenate 'string "?" (symbol-name x))
-   x))
-
-(defprojection make-symbols-ignorable (x)
-  (make-symbol-ignorable x)
-  :guard (symbol-listp x)
-  :optimize nil)
-
-(defun returnspec-thms (fnname specs world)
-  "Returns EVENTS"
-  (declare (xargs :guard (and (symbolp fnname)
-                              (returnspeclist-p specs)
-                              (plist-worldp world))))
-  (b* (((unless specs)
-        nil)
-       ((when (equal (len specs) 1))
-        (returnspec-single-thm fnname (car specs) world))
-       (names   (returnspeclist->names specs))
-       (ignorable-names (make-symbols-ignorable names))
-       (formals (look-up-formals fnname world))
-       (binds   `((mv . ,ignorable-names) (,fnname . ,formals))))
-    (returnspec-multi-thms fnname binds specs world)))
-
 
 ; -------------- Main Stuff Parsing -------------------------------------------
 
-(defund split-/// (fnname x)
-  "Returns (mv main-stuff rest-events)"
-  (declare (xargs :guard t))
-  (b* (((when (not x))
-        (mv nil nil))
-       ((when (atom x))
-        (er hard? 'split-///
-            "Expected arguments to (~x0 ~x1 ...) to be nil-terminated, but ~
-             found ~x2." 'define fnname x)
-        (mv nil nil))
-       ((when (eq (car x) '///))
-        (mv nil (cdr x)))
-       ((mv main-stuff rest-events)
-        (split-/// fnname (cdr x))))
-    (mv (cons (car x) main-stuff) rest-events)))
-
-(defthm true-listp-of-split-///-0
-  (true-listp (mv-nth 0 (split-/// fnname x)))
-  :rule-classes :type-prescription
-  :hints(("Goal" :in-theory (enable split-///))))
-
-(defthm true-listp-of-split-///-1
-  (implies (true-listp x)
-           (true-listp (mv-nth 1 (split-/// fnname x))))
-  :rule-classes :type-prescription
-  :hints(("Goal" :in-theory (enable split-///))))
-
-(defund get-xargs-from-kwd-alist (kwd-alist)
+(defun get-xargs-from-kwd-alist (kwd-alist)
   "Returns (mv xarg-stuff rest-of-kwd-alist)"
   (declare (xargs :guard (alistp kwd-alist)))
   (b* (((when (atom kwd-alist))
@@ -1433,15 +305,7 @@ some kind of separator!</p>
         (mv (list* key1 val1 xarg-stuff) kwd-alist)))
     (mv xarg-stuff (acons key1 val1 kwd-alist))))
 
-(defthm alistp-of-get-xargs-from-kwd-alist
-  (implies (force (alistp kwd-alist))
-           (b* (((mv ?xarg-stuff kwd-alist)
-                 (get-xargs-from-kwd-alist kwd-alist)))
-             (alistp kwd-alist)))
-  :hints(("Goal" :in-theory (enable get-xargs-from-kwd-alist))))
-
-
-(defund get-before-events-from-kwd-alist (kwd-alist)
+(defun get-before-events-from-kwd-alist (kwd-alist)
   "Returns (mv events rest-of-kwd-alist)"
   (declare (xargs :guard (alistp kwd-alist)))
   (b* (((when (atom kwd-alist))
@@ -1455,20 +319,7 @@ some kind of separator!</p>
         (mv (cons `(set-irrelevant-formals-ok ,val1) events) kwd-alist)))
     (mv events (acons key1 val1 kwd-alist))))
 
-(defthm true-listp-of-get-before-events-from-kwd-alist
-  (true-listp (mv-nth 0 (get-before-events-from-kwd-alist kwd-alist)))
-  :rule-classes :type-prescription
-  :hints(("Goal" :in-theory (enable get-before-events-from-kwd-alist))))
-
-(defthm alistp-of-get-before-events-from-kwd-alist
-  (implies (force (alistp kwd-alist))
-           (b* (((mv ?xarg-stuff kwd-alist)
-                 (get-before-events-from-kwd-alist kwd-alist)))
-             (alistp kwd-alist)))
-  :hints(("Goal" :in-theory (enable get-before-events-from-kwd-alist))))
-
-
-(defund get-xdoc-stuff (kwd-alist)
+(defun get-xdoc-stuff (kwd-alist)
   "Returns (mv parents short long rest-of-kwd-alist)"
   (declare (xargs :guard (alistp kwd-alist)))
   (b* ((parents (cdr (assoc :parents kwd-alist)))
@@ -1479,14 +330,7 @@ some kind of separator!</p>
        (kwd-alist (delete-assoc :long kwd-alist)))
     (mv parents short long kwd-alist)))
 
-(defthm alistp-of-get-xdoc-stuff
-  (implies (force (alistp kwd-alist))
-           (b* (((mv ?parents ?short ?long kwd-alist)
-                 (get-xdoc-stuff kwd-alist)))
-             (alistp kwd-alist)))
-  :hints(("Goal" :in-theory (enable get-xdoc-stuff))))
-
-(defund get-defun-params (kwd-alist)
+(defun get-defun-params (kwd-alist)
   "Returns (mv enabled-p inline-p prepwork rest-of-kwd-alist)"
   (declare (xargs :guard (alistp kwd-alist)))
   (b* ((enabled-p (cdr (assoc :enabled kwd-alist)))
@@ -1497,14 +341,7 @@ some kind of separator!</p>
        (kwd-alist (delete-assoc :prepwork kwd-alist)))
     (mv enabled-p inline-p prepwork kwd-alist)))
 
-(defthm alistp-of-get-defun-params
-  (implies (force (alistp kwd-alist))
-           (b* (((mv ?enabled-p ?inline-p ?prepwork kwd-alist)
-                 (get-defun-params kwd-alist)))
-             (alistp kwd-alist)))
-  :hints(("Goal" :in-theory (enable get-defun-params))))
-
-(defund get-assertion (kwd-alist)
+(defun get-assertion (kwd-alist)
   "Returns (mv assertion rest-of-kwd-alist)"
   (declare (xargs :guard (alistp kwd-alist)))
   (b* ((assertion (cdr (assoc :assert kwd-alist)))
@@ -1514,26 +351,13 @@ some kind of separator!</p>
        (kwd-alist (delete-assoc :assert kwd-alist)))
     (mv assertion kwd-alist)))
 
-(defthm alistp-of-get-assertion
-  (implies (force (alistp kwd-alist))
-           (b* (((mv ?assertion kwd-alist)
-                 (get-assertion kwd-alist)))
-             (alistp kwd-alist)))
-  :hints(("Goal" :in-theory (enable get-assertion))))
-
-(defund get-returns (kwd-alist)
+(defun get-returns (kwd-alist)
   "Returns (mv returns rest-of-kwd-alist)"
   (declare (xargs :guard (alistp kwd-alist)))
   (b* ((returns   (cdr (assoc :returns kwd-alist)))
        (kwd-alist (delete-assoc :returns kwd-alist)))
     (mv returns kwd-alist)))
 
-(defthm alistp-of-get-returns
-  (implies (force (alistp kwd-alist))
-           (b* (((mv ?returns kwd-alist)
-                 (get-returns kwd-alist)))
-             (alistp kwd-alist)))
-  :hints(("Goal" :in-theory (enable get-returns))))
 
 (defconst *define-keywords*
   (append '(:ignore-ok
@@ -1563,7 +387,7 @@ some kind of separator!</p>
 ; values there are, and if any of them are stobj names they'll have names.
 ; This will also let us double-check the return value arities.
 
-(defund nils-to-stars (x)
+(defun nils-to-stars (x)
   (declare (xargs :guard t))
   (cond ((atom x)
          nil)
@@ -1572,12 +396,7 @@ some kind of separator!</p>
         (t
          (cons (car x) (nils-to-stars (cdr x))))))
 
-(defthm symbol-listp-of-nils-to-stars
-  (implies (symbol-listp x)
-           (symbol-listp (nils-to-stars x)))
-  :hints(("Goal" :in-theory (enable nils-to-stars))))
-
-(defund return-value-names (fnname returnspecs world)
+(defun return-value-names (fnname returnspecs world)
   (declare (xargs :guard (and (symbolp fnname)
                               (returnspeclist-p returnspecs)
                               (plist-worldp world))))
@@ -1602,7 +421,6 @@ some kind of separator!</p>
    acc                ; accumulator for chars in reverse order
    state)
   "Returns (mv acc state)"
-  (declare (xargs :mode :program))
   (b* ((args (look-up-wrapper-args wrapper (w state)))
        (call-sexpr (cons wrapper args))
        (ret-sexpr (cond ((atom return-value-names)
@@ -1618,7 +436,7 @@ some kind of separator!</p>
        ((mv ret-str state)  (xdoc::fmt-to-str ret-sexpr base-pkg state))
        (call-len (length call-str)) ;; sensible since not yet encoded
        (ret-len  (length ret-str))  ;; sensible since not yet encoded
-       (acc (str::revappend-chars "<box><p><b>Signature:</b>" acc))
+       (acc (str::revappend-chars "<dt>Signature</dt><dt>" acc))
        (acc (if (< (+ call-len ret-len) 60)
                 ;; Short signature, so put it all on the same line.  I'm still
                 ;; going to use <code> instead of <tt>, for consistency.
@@ -1639,29 +457,17 @@ some kind of separator!</p>
                    (acc (xdoc::simple-html-encode-str ret-str 0 ret-len acc))
                    (acc (str::revappend-chars "</code>" acc)))
                 acc)))
-       (acc (str::revappend-chars "</p></box>" acc)))
+       (acc (str::revappend-chars "</dt>" acc)))
     (mv acc state)))
 
-(defsection ends-with-period-p
 
-  (defun ends-with-period-p (x)
-    (let ((xl (length x)))
-      (and (> xl 0)
-           (eql (char x (- (length x) 1)) #\.))))
-
-  (local
-   (progn
-    (assert! (not (ends-with-period-p "")))
-    (assert! (not (ends-with-period-p "foo")))
-    (assert! (ends-with-period-p "foo.")))))
-
-(defund formal-can-generate-doc-p (x)
+(defun formal-can-generate-doc-p (x)
   (declare (xargs :guard (formal-p x)))
   (b* (((formal x) x))
     (or (not (equal x.doc ""))
         (not (eq x.guard t)))))
 
-(defund formals-can-generate-doc-p (x)
+(defun formals-can-generate-doc-p (x)
   (declare (xargs :guard (formallist-p x)))
   (if (atom x)
       nil
@@ -1669,8 +475,7 @@ some kind of separator!</p>
         (formals-can-generate-doc-p (cdr x)))))
 
 (defun doc-from-formal (x acc base-pkg state)
-  (declare (xargs :guard (formal-p x)
-                  :mode :program))
+  (declare (xargs :guard (formal-p x)))
   (b* (((formal x) x)
 
        ((unless (formal-can-generate-doc-p x))
@@ -1681,33 +486,38 @@ some kind of separator!</p>
        (acc (str::revappend-chars "<tt>" acc))
        (acc (xdoc::simple-html-encode-str name-str 0 (length name-str) acc))
        (acc (str::revappend-chars "</tt>" acc))
+       (acc (str::revappend-chars " &mdash; " acc))
 
        (acc (if (equal x.doc "")
                 acc
-              (b* ((acc (str::revappend-chars " &mdash; " acc))
-                   (acc (str::revappend-chars x.doc acc))
+              (b* ((acc (str::revappend-chars x.doc acc))
                    (acc (if (ends-with-period-p x.doc)
                             acc
                           (cons #\. acc))))
                 acc)))
 
        ((when (eq x.guard t))
-        (b* ((acc (str::revappend-chars "</dd>" acc)))
+        (b* ((acc (str::revappend-chars "</dd>" acc))
+             (acc (cons #\Newline acc)))
           (mv acc state)))
 
+       (acc (if (equal x.doc "")
+                acc
+              (str::revappend-chars "<br/>&nbsp;&nbsp;&nbsp;&nbsp;" acc)))
+       (acc (str::revappend-chars "<color rgb='#606060'>" acc))
        ((mv guard-str state) (xdoc::fmt-to-str x.guard base-pkg state))
        ;; Using @('...') here isn't necessarily correct.  If the sexpr has
        ;; something in it that can lead to '), we are hosed.  BOZO eventually
        ;; check for this and make sure we use <code> tags instead, if it
        ;; happens.
-       (acc (str::revappend-chars " Guard @('" acc))
+       (acc (str::revappend-chars "Guard @('" acc))
        (acc (str::revappend-chars guard-str acc))
-       (acc (str::revappend-chars "').</dd>" acc)))
+       (acc (str::revappend-chars "').</color></dd>" acc))
+       (acc (cons #\Newline acc)))
     (mv acc state)))
 
 (defun doc-from-formals-aux (x acc base-pkg state)
-  (declare (xargs :guard (formallist-p x)
-                  :mode :program))
+  (declare (xargs :guard (formallist-p x)))
   (b* (((when (atom x))
         (mv acc state))
        ((mv acc state)
@@ -1715,33 +525,121 @@ some kind of separator!</p>
     (doc-from-formals-aux (cdr x) acc base-pkg state)))
 
 (defun doc-from-formals (x acc base-pkg state)
-  (declare (xargs :guard (formallist-p x)
-                  :mode :program))
+  (declare (xargs :guard (formallist-p x)))
   (b* (((unless (formals-can-generate-doc-p x))
         (mv acc state))
-       (acc (str::revappend-chars "<dl><dt>Inputs</dt>" acc))
-       ((mv acc state) (doc-from-formals-aux x acc base-pkg state))
-       (acc (str::revappend-chars "</dl>" acc)))
+       (acc (str::revappend-chars "<dt>Arguments</dt>" acc))
+       ((mv acc state) (doc-from-formals-aux x acc base-pkg state)))
+    (mv acc state)))
+
+
+(defun returnspec-can-generate-doc-p (x)
+  (declare (xargs :guard (returnspec-p x)))
+  (b* (((returnspec x) x))
+    (or (not (equal x.doc ""))
+        (not (eq x.return-type t)))))
+
+(defun returnspecs-can-generate-doc-p (x)
+  (declare (xargs :guard (returnspeclist-p x)))
+  (if (atom x)
+      nil
+    (or (returnspec-can-generate-doc-p (car x))
+        (returnspecs-can-generate-doc-p (cdr x)))))
+
+(defun doc-from-returnspec (x acc base-pkg state)
+  (declare (xargs :guard (returnspec-p x)))
+  (b* (((returnspec x) x)
+
+       ((unless (returnspec-can-generate-doc-p x))
+        (mv acc state))
+
+       (acc (str::revappend-chars "<dd>" acc))
+       ((mv name-str state) (xdoc::fmt-to-str x.name base-pkg state))
+       (acc (str::revappend-chars "<tt>" acc))
+       (acc (xdoc::simple-html-encode-str name-str 0 (length name-str) acc))
+       (acc (str::revappend-chars "</tt>" acc))
+       (acc (str::revappend-chars " &mdash; " acc))
+
+       (acc (if (equal x.doc "")
+                acc
+              (b* ((acc (str::revappend-chars x.doc acc))
+                   (acc (if (ends-with-period-p x.doc)
+                            acc
+                          (cons #\. acc))))
+                acc)))
+
+       ((when (eq x.return-type t))
+        (b* ((acc (str::revappend-chars "</dd>" acc))
+             (acc (cons #\Newline acc)))
+          (mv acc state)))
+
+       (acc (if (equal x.doc "")
+                acc
+              (str::revappend-chars "<br/>&nbsp;&nbsp;&nbsp;&nbsp;" acc)))
+       (acc (str::revappend-chars "<color rgb='#606060'>" acc))
+       ((mv type-str state) (xdoc::fmt-to-str x.return-type base-pkg state))
+       ;; Using @('...') here isn't necessarily correct.  If the sexpr has
+       ;; something in it that can lead to '), we are hosed.  BOZO eventually
+       ;; check for this and make sure we use <code> tags instead, if it
+       ;; happens.
+       (acc (str::revappend-chars "Type @('" acc))
+       (acc (str::revappend-chars type-str acc))
+       (acc (str::revappend-chars "')" acc))
+       ((mv acc state)
+        (cond ((eq x.hyp t)
+               (mv (cons #\. acc) state))
+              ((or (eq x.hyp :guard)
+                   (eq x.hyp :fguard))
+               (mv (str::revappend-chars ", given the @(see guard)." acc)
+                   state))
+              (t
+               (b* ((acc (str::revappend-chars ", given @('" acc))
+                    ((mv hyp-str state)
+                     (xdoc::fmt-to-str x.hyp base-pkg state))
+                    (acc (str::revappend-chars hyp-str acc))
+                    (acc (str::revappend-chars "')." acc)))
+                 (mv acc state)))))
+       (acc (str::revappend-chars "</color>" acc))
+       (acc (str::revappend-chars "</dd>" acc))
+       (acc (cons #\Newline acc)))
+
+    (mv acc state)))
+
+(defun doc-from-returnspecs-aux (x acc base-pkg state)
+  (declare (xargs :guard (returnspeclist-p x)))
+  (b* (((when (atom x))
+        (mv acc state))
+       ((mv acc state)
+        (doc-from-returnspec (car x) acc base-pkg state)))
+    (doc-from-returnspecs-aux (cdr x) acc base-pkg state)))
+
+(defun doc-from-returnspecs (x acc base-pkg state)
+  (declare (xargs :guard (returnspeclist-p x)))
+  (b* (((unless (returnspecs-can-generate-doc-p x))
+        (mv acc state))
+       (acc (str::revappend-chars "<dt>Returns</dt>" acc))
+       ((mv acc state) (doc-from-returnspecs-aux x acc base-pkg state)))
     (mv acc state)))
 
 (defun make-xdoc-top (wrapper fnname formals returnspecs base-pkg state)
   "Returns (mv str state)"
-  (declare (xargs :mode :program))
   (b* ((world (w state))
        (acc nil)
+       (acc (str::revappend-chars "<box><dl>" acc))
+       (acc (cons #\Newline acc))
        (return-value-names (return-value-names fnname returnspecs world))
-       ((mv acc state)
-        (make-xdoc-signature wrapper return-value-names base-pkg acc state))
-       ((mv acc state)
-        (doc-from-formals formals acc base-pkg state))
-       (str (reverse (coerce acc 'string))))
+       ((mv acc state) (make-xdoc-signature wrapper return-value-names base-pkg acc state))
+       ((mv acc state) (doc-from-formals formals acc base-pkg state))
+       ((mv acc state) (doc-from-returnspecs returnspecs acc base-pkg state))
+       (acc (str::revappend-chars "</dl></box>" acc))
+       (acc (cons #\Newline acc))
+       (str (str::rchars-to-string acc)))
     (mv str state)))
-
 
 
 ; -------------- Top-Level Macro ----------------------------------------------
 
-(defund define-fn (fnname formals args world)
+(defun define-fn (fnname formals args world)
   (declare (xargs :guard (plist-worldp world)))
   (b* (((unless (symbolp fnname))
         (er hard? 'define-fn
@@ -1753,15 +651,6 @@ some kind of separator!</p>
         (extract-keywords fnname *define-keywords* main-stuff nil))
        (traditional-decls/docs (butlast normal-defun-stuff 1))
        (body          (car (last normal-defun-stuff)))
-
-;; I originally generated __function__ in a package based on the function name.
-;; The goal was to make it easy to use __function__ in other packages without
-;; having to remember to import it, etc.  But then, when I added raise, I
-;; realized how inconvenient this is.  You can't write something like raise
-;; unless you know which package __function__ will live in.  So, now, just
-;; always target cutil::__function__ which is the same as acl2::__function__
-;; and can be imported as desired.
-
        (extended-body `(let ((__function__ ',fnname))
                          ;; CCL's compiler seems to be smart enough to not
                          ;; generate code for this binding when it's not
@@ -1780,8 +669,8 @@ some kind of separator!</p>
         (er hard? 'define-fn
             "Error in ~x0: expected :assert to be either a symbol or a ~
              symbol-listp, but found ~x1."
-            fnname assertion)) 
-       (ruler-extenders (if assertion :all nil))       
+            fnname assertion))
+       (ruler-extenders (if assertion :all nil))
 
        ((unless (true-listp prepwork))
         (er hard? 'define-fn
@@ -1809,7 +698,7 @@ some kind of separator!</p>
        (macro         (and need-macrop
                            (make-wrapper-macro fnname fnname-fn formals)))
        (formals       (remove-macro-args fnname formals nil))
-       (formals       (parse-formals fnname formals))
+       (formals       (parse-formals fnname formals nil))
        (formal-names  (formallist->names formals))
        (formal-guards (remove t (formallist->guards formals)))
        (stobj-names   (formallist->names (formallist-collect-stobjs formals world)))
@@ -1979,28 +868,5 @@ some kind of separator!</p>
          'untranslate-preproc-for-define))
 
 
-(defsection raise
-  :parents (define)
-  :short "Shorthand for causing hard errors, for use in @(see define)."
 
-  :long "<p>@(call raise) is a macro that is equivalent to @('(er hard? ...)'),
-but it automatically fills in the function name using @('__function__').  So,
-rather than write something like:</p>
-
-@({
- (er hard? __function__ \"bad input value ~x0~%\" x)
-})
-
-<p>You can just write:</p>
-
-@({
- (raise \"bad input value ~x0~%\" x)
-})
-
-<p>Logically @('raise') just returns @('nil').</p>
-
-@(def raise)"
-
-  (defmacro raise (&rest args)
-    `(er hard? __function__ . ,args)))
 
