books/centaur/gl/defagg.lisp
@@ -77,6 +77,7 @@
 #!CUTIL
 (defmacro GL::defagg-fns (name fields &key tag require hons (legiblep 't)
                                (debugp 'nil))
+  (declare (ignorable debugp))
   (and (or (symbolp name)
            (er hard 'defaggregate "Name must be a symbol.~%"))
        (or (symbol-listp fields)
@@ -98,7 +99,7 @@
        (or (pseudo-term-listp (strip-cadrs require))
            (er hard 'defaggregate "The requierments must be terms.~%"))
        (let ((x (da-x name)))
-         `(progn ,(da-make-recognizer name tag fields require legiblep debugp)
+         `(progn ,(da-make-recognizer name tag fields require legiblep)
                  ;; jared: removing this, it's not included in vl anymore
                  ;; ,(da-make-debugger name tag fields require legiblep)
                  ,(da-make-constructor name tag fields require hons legiblep)
