books/centaur/vl/toe/toe-emodwire.lisp
@@ -1090,7 +1090,7 @@ index of @('|reset|') is @('nil').</p>"
 
 ;; Introduce defaggregate like make-vl-emodwire and change-vl-emodwire macros.
 
-(make-event (cutil::da-make-maker-fn 'vl-emodwire '(basename index)))
+(make-event (cutil::da-make-maker-fn 'vl-emodwire '(basename index) nil))
 (make-event (cutil::da-make-maker 'vl-emodwire '(basename index)))
 (make-event (cutil::da-make-changer-fn 'vl-emodwire '(basename index)))
 (make-event (cutil::da-make-changer 'vl-emodwire '(basename index)))
