books/cutil/support.lisp
@@ -19,25 +19,151 @@
 ; Original author: Jared Davis <jared@centtech.com>
 
 (in-package "CUTIL")
+(include-book "xdoc/top" :dir :system)
+(include-book "misc/definline" :dir :system)
 (include-book "tools/bstar" :dir :system)
 
-(defun tuplep (n x)
-  (declare (xargs :guard (natp n)))
-  (mbe :logic (and (true-listp x)
-                   (equal (len x) n))
-       :exec (and (true-listp x)
-                  (eql (length x) n))))
+(defxdoc support
+  :parents (cutil)
+  :short "Miscellaneous supporting functions.")
 
-(defun tuple-listp (n x)
-  (declare (xargs :guard (natp n)))
-  (if (consp x)
-      (and (tuplep n (car x))
-           (tuple-listp n (cdr x)))
-    t))
+(defsection tuplep
+  :parents (support)
+  :short "@(call tuplep) recognizes nil-terminated @('n')-tuples."
 
-(defun cons-listp (x)
-  (declare (xargs :guard t))
-  (if (consp x)
-      (and (consp (car x))
-           (cons-listp (cdr x)))
-    t))
+  (defun tuplep (n x)
+    (declare (xargs :guard (natp n)))
+    (mbe :logic (and (true-listp x)
+                     (equal (len x) n))
+         :exec (and (true-listp x)
+                    (eql (length x) n)))))
+
+(defsection tuple-listp
+  :parents (support)
+  :short "@(call tuple-listp) recognizes a list of nil-terminated @('n')-tuples."
+
+  (defun tuple-listp (n x)
+    (declare (xargs :guard (natp n)))
+    (if (consp x)
+        (and (tuplep n (car x))
+             (tuple-listp n (cdr x)))
+      t)))
+
+(defsection cons-listp
+  :parents (support)
+  :short "@(call cons-listp) is like @(see alistp) but does not require the
+list to be nil-terminated."
+
+  (defun cons-listp (x)
+    (declare (xargs :guard t))
+    (if (consp x)
+        (and (consp (car x))
+             (cons-listp (cdr x)))
+      t)))
+
+
+
+(defsection raise
+  :parents (support define)
+  :short "Shorthand for causing hard errors."
+
+  :long "<p>@(call raise) is equivalent to @('(er hard? ...)'), but it
+automatically fills in the function name using @('__function__').  This only
+works in contexts where @('__function__') is bound, e.g., the body of a @(see
+define) or within a @(see defconsts) form.  In these contexts, rather than
+write something like:</p>
+
+@({
+ (er hard? __function__ \"bad input value ~x0~%\" x)
+})
+
+<p>You can just write:</p>
+
+@({
+ (raise \"bad input value ~x0~%\" x)
+})
+
+<p>Logically @('raise') just returns @('nil').</p>
+
+@(def raise)"
+
+  (defmacro raise (&rest args)
+    `(er hard? __function__ . ,args)))
+
+
+
+(program)
+
+(defsection extract-keywords
+  :parents (support)
+  :short "Extract legal keyword/value pairs from an argument list."
+
+  (defun extract-keywords
+    (ctx        ; context for error messages
+     legal-kwds ; what keywords the args are allowed to contain
+     args       ; args that the user supplied
+     kwd-alist  ; accumulator alist of extracted keywords to values
+     )
+  "Returns (mv kwd-alist other-args)"
+  (declare (xargs :guard (and (symbol-listp legal-kwds)
+                              (no-duplicatesp legal-kwds)
+                              (alistp kwd-alist))))
+  (b* ((__function__ 'extract-keywords)
+       ((when (atom args))
+        (mv kwd-alist args))
+       (arg1 (first args))
+       ((unless (keywordp arg1))
+        (b* (((mv kwd-alist other-args)
+              (extract-keywords ctx legal-kwds (cdr args) kwd-alist)))
+          (mv kwd-alist (cons arg1 other-args))))
+       ((unless (member arg1 legal-kwds))
+        (raise (concatenate 'string
+                            "~x0: invalid keyword ~x1."
+                            (if legal-kwds
+                                "  Valid keywords: ~&2."
+                              "  No keywords are valid here."))
+               ctx arg1 legal-kwds)
+        (mv nil nil))
+       ((when (atom (rest args)))
+        (raise "~x0: keyword ~x1 has no argument." ctx arg1)
+        (mv nil nil))
+       ((when (assoc arg1 kwd-alist))
+        (raise "~x0: multiple occurrences of keyword ~x1." ctx arg1)
+        (mv nil nil))
+       (value (second args))
+       (kwd-alist (acons arg1 value kwd-alist)))
+    (extract-keywords ctx legal-kwds (cddr args) kwd-alist))))
+
+(defsection split-///
+  :parents (support)
+  :short "Split an argument list into pre- and post-@('///') contents."
+
+  (defun split-/// (ctx x)
+    "Returns (mv pre-/// post-///)"
+    (declare (xargs :guard t))
+    (b* ((__function__ 'split-///)
+         ((when (not x))
+          (mv nil nil))
+         ((when (atom x))
+          (raise "~x0: expected nil-terminated arguments but found ~x1." ctx x)
+          (mv nil nil))
+         ((when (eq (car x) '///))
+          (mv nil (cdr x)))
+         ((mv pre post)
+          (split-/// ctx (cdr x))))
+      (mv (cons (car x) pre) post))))
+
+
+(defsection ends-with-period-p
+  :parents (support)
+  :short "Determines if a string ends with a period."
+
+  (defun ends-with-period-p (x)
+    (declare (xargs :guard (stringp x)))
+    (let ((xl (length x)))
+      (and (> xl 0)
+           (eql (char x (- (length x) 1)) #\.)))))
+
+
+
+
